update

Coq Scripts/Definitions.v
@@ -1,19 +1,51 @@
+Class aDecSet (X : Set) : Set :=
+  eq_dec : forall x y : X, {x = y} + {x <> y}.
+
+
 Structure Program :=
 { datatype : Set
+; datatype_aDecSet : aDecSet datatype
 ; algorithm : datatype -> option datatype
 }.
 
 
 Inductive pass (p : Program) : datatype p -> datatype p -> Prop :=
-| refl : forall x : datatype p, pass p x x
-| cont : forall x x' y : datatype p,
-	pass p x x' -> algorithm p x' = Some y -> pass p x y.
+| step : forall x y : datatype p, algorithm p x = Some y -> pass p x y
+| trans : forall x y z : datatype p,
+	  pass p x y -> pass p y z -> pass p x z.
 
 Notation "p : x ==> y" := (pass p x y) (at level 70).
 
 
 Definition compute (p : Program) : datatype p -> datatype p -> Prop :=
-  fun x y => forall x y, p : x ==> y /\ algorithm p y = None.
+  fun x y => p : x ==> y /\ algorithm p y = None.
 
 Notation "p : x ==>! y" := (compute p x y) (at level 70).
- 
+
+
+Section nsteps.
+Variable p : Program.
+Variables x y : datatype p.
+Hypothesis H : p : x ==> y.
+
+Fixpoint nsteps : nat :=  
+
+
+
+Lemma Church_Rosser :
+  forall p x y1 y2, p : x ==> y1 -> p : x ==> y2 ->
+    exists z, p : y1 ==> z /\ p : y2 ==> z.
+Proof.
+  intros.
+
+Lemma func_compute : forall (p : Program) (x y z : datatype p),
+  p : x ==>! y -> p : x ==>! z -> y = z.
+Proof.
+  intros *. unfold "_ : _ ==>! _". intros Hy Hz.
+  destruct Hy as (Hy, Hy'). destruct Hz as (Hz, Hz').
+  destruct Hy as [| x y' y Hxy' Hy'y].
+  - 
+  induction Hz as [x z Hxz | x z' z Hxz' Hz'z].
+  - rewrite H in Hxz. now injection Hxz.
+  - apply IHHz1. 2: { trivial. }
+     
